\section{Models of Memory}

Ebbinghaus \cite{ebbinghaus} 
\ldots

\begin{equation}
\label{eq:ebbinghaus}
 S(t) = ae^{-bt}
\end{equation}

If $a=1$, this may be interpreted as a probability function:

\begin{equation}
\label{eq:ebbinghaus}
 p(t) = e^{-bt}
\end{equation}

\section{ACT-R}

John Anderson \cite{anderson} 
\ldots

\section{Updates to Memory Model}

\begin{equation}
\label{eq:ebbinghaus}
 p(t) = \frac{1}{1 + e^{m(t-\lambda)}}
\end{equation}

% TODO: memory figure

\section{Re-Activation}

\begin{equation}
\label{eq:ebbinghaus}
 \lambda_n = \rho \lambda_{n-1}
\end{equation}

\subsection{Spacing Effect}
